bump to nightly-2023-02-02-22
mathlib commit https://github.com/leanprover-community/mathlib/commit/d90e4e186f1d18e375dcd4e5b5f6364b01cb3e46

Mathbin/SetTheory/Lists.lean
@@ -48,6 +48,7 @@ The next step is to define ZFA sets as lists quotiented by `lists.equiv`.
 
 variable {α : Type _}
 
+#print Lists' /-
 /-- Prelists, helper type to define `lists`. `lists' α ff` are the "atoms", a copy of `α`.
 `lists' α tt` are the "proper" ZFA prelists, inductively defined from the empty ZFA prelist and from
 appending a ZFA prelist to a proper ZFA prelist. It is made so that you can't append anything to an
@@ -59,13 +60,16 @@ inductive Lists'.{u} (α : Type u) : Bool → Type u
   | cons' {b} : Lists' b → Lists' true → Lists' true
   deriving DecidableEq
 #align lists' Lists'
+-/
 
+#print Lists /-
 /-- Hereditarily finite list, aka ZFA list. A ZFA list is either an "atom" (`b = ff`), corresponding
 to an element of `α`, or a "proper" ZFA list, inductively defined from the empty ZFA list and from
 appending a ZFA list to a proper ZFA list. -/
 def Lists (α : Type _) :=
   Σb, Lists' α b
 #align lists Lists
+-/
 
 namespace Lists'
 
@@ -73,11 +77,14 @@ instance [Inhabited α] : ∀ b, Inhabited (Lists' α b)
   | tt => ⟨nil⟩
   | ff => ⟨atom default⟩
 
+#print Lists'.cons /-
 /-- Appending a ZFA list to a proper ZFA prelist. -/
 def cons : Lists α → Lists' α true → Lists' α true
   | ⟨b, a⟩, l => cons' a l
 #align lists'.cons Lists'.cons
+-/
 
+#print Lists'.toList /-
 /-- Converts a ZFA prelist to a `list` of ZFA lists. Atoms are sent to `[]`. -/
 @[simp]
 def toList : ∀ {b}, Lists' α b → List (Lists α)
@@ -85,23 +92,31 @@ def toList : ∀ {b}, Lists' α b → List (Lists α)
   | _, nil => []
   | _, cons' a l => ⟨_, a⟩ :: l.toList
 #align lists'.to_list Lists'.toList
+-/
 
+#print Lists'.toList_cons /-
 @[simp]
 theorem toList_cons (a : Lists α) (l) : toList (cons a l) = a :: l.toList := by
   cases a <;> simp [cons]
 #align lists'.to_list_cons Lists'.toList_cons
+-/
 
+#print Lists'.ofList /-
 /-- Converts a `list` of ZFA lists to a proper ZFA prelist. -/
 @[simp]
 def ofList : List (Lists α) → Lists' α true
   | [] => nil
   | a :: l => cons a (of_list l)
 #align lists'.of_list Lists'.ofList
+-/
 
+#print Lists'.to_ofList /-
 @[simp]
 theorem to_ofList (l : List (Lists α)) : toList (ofList l) = l := by induction l <;> simp [*]
 #align lists'.to_of_list Lists'.to_ofList
+-/
 
+#print Lists'.of_toList /-
 @[simp]
 theorem of_toList : ∀ l : Lists' α true, ofList (toList l) = l :=
   suffices
@@ -115,9 +130,11 @@ theorem of_toList : ∀ l : Lists' α true, ofList (toList l) = l :=
     intro ; change l' with cons' a l
     simpa [cons] using IH₂ rfl
 #align lists'.of_to_list Lists'.of_toList
+-/
 
 end Lists'
 
+#print Lists.Equiv /-
 mutual
   inductive Lists.Equiv : Lists α → Lists α → Prop
     | refl (l) : Lists.Equiv l l
@@ -133,6 +150,7 @@ mutual
 end
 #align lists.equiv Lists.Equiv
 #align lists'.subset Lists'.Subset
+-/
 
 -- mathport name: «expr ~ »
 local infixl:50 " ~ " => Lists.Equiv
@@ -153,15 +171,33 @@ equivalent as a ZFA list to this ZFA list. -/
 instance {b} : Membership (Lists α) (Lists' α b) :=
   ⟨fun a l => ∃ a' ∈ l.toList, a ~ a'⟩
 
+/- warning: lists'.mem_def -> Lists'.mem_def is a dubious translation:
+lean 3 declaration is
+  forall {α : Type.{u1}} {b : Bool} {a : Lists.{u1} α} {l : Lists'.{u1} α b}, Iff (Membership.Mem.{u1, u1} (Lists.{u1} α) (Lists'.{u1} α b) (Lists'.hasMem.{u1} α b) a l) (Exists.{succ u1} (Lists.{u1} α) (fun (a' : Lists.{u1} α) => Exists.{0} (Membership.Mem.{u1, u1} (Lists.{u1} α) (List.{u1} (Lists.{u1} α)) (List.hasMem.{u1} (Lists.{u1} α)) a' (Lists'.toList.{u1} α b l)) (fun (H : Membership.Mem.{u1, u1} (Lists.{u1} α) (List.{u1} (Lists.{u1} α)) (List.hasMem.{u1} (Lists.{u1} α)) a' (Lists'.toList.{u1} α b l)) => Lists.Equiv.{u1} α a a')))
+but is expected to have type
+  forall {α : Type.{u1}} {b : Bool} {a : Lists.{u1} α} {l : Lists'.{u1} α b}, Iff (Membership.mem.{u1, u1} (Lists.{u1} α) (Lists'.{u1} α b) (Lists'.instMembershipListsLists'.{u1} α b) a l) (Exists.{succ u1} (Lists.{u1} α) (fun (a' : Lists.{u1} α) => And (Membership.mem.{u1, u1} (Lists.{u1} α) (List.{u1} (Lists.{u1} α)) (List.instMembershipList.{u1} (Lists.{u1} α)) a' (Lists'.toList.{u1} α b l)) (Lists.Equiv.{u1} α a a')))
+Case conversion may be inaccurate. Consider using '#align lists'.mem_def Lists'.mem_defₓ'. -/
 theorem mem_def {b a} {l : Lists' α b} : a ∈ l ↔ ∃ a' ∈ l.toList, a ~ a' :=
   Iff.rfl
 #align lists'.mem_def Lists'.mem_def
 
+/- warning: lists'.mem_cons -> Lists'.mem_cons is a dubious translation:
+lean 3 declaration is
+  forall {α : Type.{u1}} {a : Lists.{u1} α} {y : Lists.{u1} α} {l : Lists'.{u1} α Bool.true}, Iff (Membership.Mem.{u1, u1} (Lists.{u1} α) (Lists'.{u1} α Bool.true) (Lists'.hasMem.{u1} α Bool.true) a (Lists'.cons.{u1} α y l)) (Or (Lists.Equiv.{u1} α a y) (Membership.Mem.{u1, u1} (Lists.{u1} α) (Lists'.{u1} α Bool.true) (Lists'.hasMem.{u1} α Bool.true) a l))
+but is expected to have type
+  forall {α : Type.{u1}} {a : Lists.{u1} α} {y : Lists.{u1} α} {l : Lists'.{u1} α Bool.true}, Iff (Membership.mem.{u1, u1} (Lists.{u1} α) (Lists'.{u1} α Bool.true) (Lists'.instMembershipListsLists'.{u1} α Bool.true) a (Lists'.cons.{u1} α y l)) (Or (Lists.Equiv.{u1} α a y) (Membership.mem.{u1, u1} (Lists.{u1} α) (Lists'.{u1} α Bool.true) (Lists'.instMembershipListsLists'.{u1} α Bool.true) a l))
+Case conversion may be inaccurate. Consider using '#align lists'.mem_cons Lists'.mem_consₓ'. -/
 @[simp]
 theorem mem_cons {a y l} : a ∈ @cons α y l ↔ a ~ y ∨ a ∈ l := by
   simp [mem_def, or_and_right, exists_or]
 #align lists'.mem_cons Lists'.mem_cons
 
+/- warning: lists'.cons_subset -> Lists'.cons_subset is a dubious translation:
+lean 3 declaration is
+  forall {α : Type.{u1}} {a : Lists.{u1} α} {l₁ : Lists'.{u1} α Bool.true} {l₂ : Lists'.{u1} α Bool.true}, Iff (HasSubset.Subset.{u1} (Lists'.{u1} α Bool.true) (Lists'.hasSubset.{u1} α) (Lists'.cons.{u1} α a l₁) l₂) (And (Membership.Mem.{u1, u1} (Lists.{u1} α) (Lists'.{u1} α Bool.true) (Lists'.hasMem.{u1} α Bool.true) a l₂) (HasSubset.Subset.{u1} (Lists'.{u1} α Bool.true) (Lists'.hasSubset.{u1} α) l₁ l₂))
+but is expected to have type
+  forall {α : Type.{u1}} {a : Lists.{u1} α} {l₁ : Lists'.{u1} α Bool.true} {l₂ : Lists'.{u1} α Bool.true}, Iff (HasSubset.Subset.{u1} (Lists'.{u1} α Bool.true) (Lists'.instHasSubsetLists'True.{u1} α) (Lists'.cons.{u1} α a l₁) l₂) (And (Membership.mem.{u1, u1} (Lists.{u1} α) (Lists'.{u1} α Bool.true) (Lists'.instMembershipListsLists'.{u1} α Bool.true) a l₂) (HasSubset.Subset.{u1} (Lists'.{u1} α Bool.true) (Lists'.instHasSubsetLists'True.{u1} α) l₁ l₂))
+Case conversion may be inaccurate. Consider using '#align lists'.cons_subset Lists'.cons_subsetₓ'. -/
 theorem cons_subset {a} {l₁ l₂ : Lists' α true} : Lists'.cons a l₁ ⊆ l₂ ↔ a ∈ l₂ ∧ l₁ ⊆ l₂ :=
   by
   refine' ⟨fun h => _, fun ⟨⟨a', m, e⟩, s⟩ => subset.cons e m s⟩
@@ -172,25 +208,37 @@ theorem cons_subset {a} {l₁ l₂ : Lists' α true} : Lists'.cons a l₁ ⊆ l�
   cases a; cases a'; cases h'; exact ⟨⟨_, m, e⟩, s⟩
 #align lists'.cons_subset Lists'.cons_subset
 
+#print Lists'.ofList_subset /-
 theorem ofList_subset {l₁ l₂ : List (Lists α)} (h : l₁ ⊆ l₂) :
     Lists'.ofList l₁ ⊆ Lists'.ofList l₂ := by
   induction l₁; · exact subset.nil
   refine' subset.cons (Lists.Equiv.refl _) _ (l₁_ih (List.subset_of_cons_subset h))
   simp at h; simp [h]
 #align lists'.of_list_subset Lists'.ofList_subset
+-/
 
+#print Lists'.Subset.refl /-
 @[refl]
 theorem Subset.refl {l : Lists' α true} : l ⊆ l := by
   rw [← Lists'.of_toList l] <;> exact of_list_subset (List.Subset.refl _)
 #align lists'.subset.refl Lists'.Subset.refl
+-/
 
+#print Lists'.subset_nil /-
 theorem subset_nil {l : Lists' α true} : l ⊆ Lists'.nil → l = Lists'.nil :=
   by
   rw [← of_to_list l]
   induction to_list l <;> intro h; · rfl
   rcases cons_subset.1 h with ⟨⟨_, ⟨⟩, _⟩, _⟩
 #align lists'.subset_nil Lists'.subset_nil
+-/
 
+/- warning: lists'.mem_of_subset' -> Lists'.mem_of_subset' is a dubious translation:
+lean 3 declaration is
+  forall {α : Type.{u1}} {a : Lists.{u1} α} {l₁ : Lists'.{u1} α Bool.true} {l₂ : Lists'.{u1} α Bool.true}, (HasSubset.Subset.{u1} (Lists'.{u1} α Bool.true) (Lists'.hasSubset.{u1} α) l₁ l₂) -> (Membership.Mem.{u1, u1} (Lists.{u1} α) (List.{u1} (Lists.{u1} α)) (List.hasMem.{u1} (Lists.{u1} α)) a (Lists'.toList.{u1} α Bool.true l₁)) -> (Membership.Mem.{u1, u1} (Lists.{u1} α) (Lists'.{u1} α Bool.true) (Lists'.hasMem.{u1} α Bool.true) a l₂)
+but is expected to have type
+  forall {α : Type.{u1}} {a : Lists.{u1} α} {l₁ : Lists'.{u1} α Bool.true} {l₂ : Lists'.{u1} α Bool.true}, (HasSubset.Subset.{u1} (Lists'.{u1} α Bool.true) (Lists'.instHasSubsetLists'True.{u1} α) l₁ l₂) -> (Membership.mem.{u1, u1} (Lists.{u1} α) (List.{u1} (Lists.{u1} α)) (List.instMembershipList.{u1} (Lists.{u1} α)) a (Lists'.toList.{u1} α Bool.true l₁)) -> (Membership.mem.{u1, u1} (Lists.{u1} α) (Lists'.{u1} α Bool.true) (Lists'.instMembershipListsLists'.{u1} α Bool.true) a l₂)
+Case conversion may be inaccurate. Consider using '#align lists'.mem_of_subset' Lists'.mem_of_subset'ₓ'. -/
 theorem mem_of_subset' {a} {l₁ l₂ : Lists' α true} (s : l₁ ⊆ l₂) (h : a ∈ l₁.toList) : a ∈ l₂ :=
   by
   induction' s with _ a a' l l' e m s IH; · cases h
@@ -198,6 +246,12 @@ theorem mem_of_subset' {a} {l₁ l₂ : Lists' α true} (s : l₁ ⊆ l₂) (h :
   exacts[⟨_, m, e⟩, IH h]
 #align lists'.mem_of_subset' Lists'.mem_of_subset'
 
+/- warning: lists'.subset_def -> Lists'.subset_def is a dubious translation:
+lean 3 declaration is
+  forall {α : Type.{u1}} {l₁ : Lists'.{u1} α Bool.true} {l₂ : Lists'.{u1} α Bool.true}, Iff (HasSubset.Subset.{u1} (Lists'.{u1} α Bool.true) (Lists'.hasSubset.{u1} α) l₁ l₂) (forall (a : Lists.{u1} α), (Membership.Mem.{u1, u1} (Lists.{u1} α) (List.{u1} (Lists.{u1} α)) (List.hasMem.{u1} (Lists.{u1} α)) a (Lists'.toList.{u1} α Bool.true l₁)) -> (Membership.Mem.{u1, u1} (Lists.{u1} α) (Lists'.{u1} α Bool.true) (Lists'.hasMem.{u1} α Bool.true) a l₂))
+but is expected to have type
+  forall {α : Type.{u1}} {l₁ : Lists'.{u1} α Bool.true} {l₂ : Lists'.{u1} α Bool.true}, Iff (HasSubset.Subset.{u1} (Lists'.{u1} α Bool.true) (Lists'.instHasSubsetLists'True.{u1} α) l₁ l₂) (forall (a : Lists.{u1} α), (Membership.mem.{u1, u1} (Lists.{u1} α) (List.{u1} (Lists.{u1} α)) (List.instMembershipList.{u1} (Lists.{u1} α)) a (Lists'.toList.{u1} α Bool.true l₁)) -> (Membership.mem.{u1, u1} (Lists.{u1} α) (Lists'.{u1} α Bool.true) (Lists'.instMembershipListsLists'.{u1} α Bool.true) a l₂))
+Case conversion may be inaccurate. Consider using '#align lists'.subset_def Lists'.subset_defₓ'. -/
 theorem subset_def {l₁ l₂ : Lists' α true} : l₁ ⊆ l₂ ↔ ∀ a ∈ l₁.toList, a ∈ l₂ :=
   ⟨fun H a => mem_of_subset' H, fun H =>
     by
@@ -212,44 +266,60 @@ end Lists'
 
 namespace Lists
 
+#print Lists.atom /-
 /-- Sends `a : α` to the corresponding atom in `lists α`. -/
 @[match_pattern]
 def atom (a : α) : Lists α :=
   ⟨_, Lists'.atom a⟩
 #align lists.atom Lists.atom
+-/
 
+#print Lists.of' /-
 /-- Converts a proper ZFA prelist to a ZFA list. -/
 @[match_pattern]
 def of' (l : Lists' α true) : Lists α :=
   ⟨_, l⟩
 #align lists.of' Lists.of'
+-/
 
+#print Lists.toList /-
 /-- Converts a ZFA list to a `list` of ZFA lists. Atoms are sent to `[]`. -/
 @[simp]
 def toList : Lists α → List (Lists α)
   | ⟨b, l⟩ => l.toList
 #align lists.to_list Lists.toList
+-/
 
+#print Lists.IsList /-
 /-- Predicate stating that a ZFA list is proper. -/
 def IsList (l : Lists α) : Prop :=
   l.1
 #align lists.is_list Lists.IsList
+-/
 
+#print Lists.ofList /-
 /-- Converts a `list` of ZFA lists to a ZFA list. -/
 def ofList (l : List (Lists α)) : Lists α :=
   of' (Lists'.ofList l)
 #align lists.of_list Lists.ofList
+-/
 
-theorem isList_to_list (l : List (Lists α)) : IsList (ofList l) :=
+#print Lists.isList_toList /-
+theorem isList_toList (l : List (Lists α)) : IsList (ofList l) :=
   Eq.refl _
-#align lists.is_list_to_list Lists.isList_to_list
+#align lists.is_list_to_list Lists.isList_toList
+-/
 
+#print Lists.to_ofList /-
 theorem to_ofList (l : List (Lists α)) : toList (ofList l) = l := by simp [of_list, of']
 #align lists.to_of_list Lists.to_ofList
+-/
 
+#print Lists.of_toList /-
 theorem of_toList : ∀ {l : Lists α}, IsList l → ofList (toList l) = l
   | ⟨tt, l⟩, _ => by simp [of_list, of']
 #align lists.of_to_list Lists.of_toList
+-/
 
 instance : Inhabited (Lists α) :=
   ⟨of' Lists'.nil⟩
@@ -258,6 +328,7 @@ instance [DecidableEq α] : DecidableEq (Lists α) := by unfold Lists <;> infer_
 
 instance [SizeOf α] : SizeOf (Lists α) := by unfold Lists <;> infer_instance
 
+#print Lists.inductionMut /-
 /-- A recursion principle for pairs of ZFA lists and proper ZFA prelists. -/
 def inductionMut (C : Lists α → Sort _) (D : Lists' α true → Sort _) (C0 : ∀ a, C (atom a))
     (C1 : ∀ l, D l → C (of' l)) (D0 : D Lists'.nil) (D1 : ∀ a l, C a → D l → D (Lists'.cons a l)) :
@@ -278,39 +349,51 @@ def inductionMut (C : Lists α → Sort _) (D : Lists' α true → Sort _) (C0 :
     · exact ⟨C1 _ this, this⟩
     exact D1 ⟨_, _⟩ _ IH₁.1 IH₂.2
 #align lists.induction_mut Lists.inductionMut
+-/
 
+#print Lists.mem /-
 /-- Membership of ZFA list. A ZFA list belongs to a proper ZFA list if it belongs to the latter as a
 proper ZFA prelist. An atom has no members. -/
-def Mem (a : Lists α) : Lists α → Prop
+def mem (a : Lists α) : Lists α → Prop
   | ⟨ff, l⟩ => False
   | ⟨tt, l⟩ => a ∈ l
-#align lists.mem Lists.Mem
+#align lists.mem Lists.mem
+-/
 
 instance : Membership (Lists α) (Lists α) :=
-  ⟨Mem⟩
+  ⟨mem⟩
 
-theorem isList_of_mem {a : Lists α} : ∀ {l : Lists α}, a ∈ l → IsList l
+#print Lists.is_list_of_mem /-
+theorem is_list_of_mem {a : Lists α} : ∀ {l : Lists α}, a ∈ l → IsList l
   | ⟨_, Lists'.nil⟩, _ => rfl
   | ⟨_, Lists'.cons' _ _⟩, _ => rfl
-#align lists.is_list_of_mem Lists.isList_of_mem
+#align lists.is_list_of_mem Lists.is_list_of_mem
+-/
 
+#print Lists.Equiv.antisymm_iff /-
 theorem Equiv.antisymm_iff {l₁ l₂ : Lists' α true} : of' l₁ ~ of' l₂ ↔ l₁ ⊆ l₂ ∧ l₂ ⊆ l₁ :=
   by
   refine' ⟨fun h => _, fun ⟨h₁, h₂⟩ => equiv.antisymm h₁ h₂⟩
   cases' h with _ _ _ h₁ h₂
   · simp [Lists'.Subset.refl]; · exact ⟨h₁, h₂⟩
 #align lists.equiv.antisymm_iff Lists.Equiv.antisymm_iff
+-/
 
 attribute [refl] Equiv.refl
 
+#print Lists.equiv_atom /-
 theorem equiv_atom {a} {l : Lists α} : atom a ~ l ↔ atom a = l :=
   ⟨fun h => by cases h <;> rfl, fun h => h ▸ Equiv.refl _⟩
 #align lists.equiv_atom Lists.equiv_atom
+-/
 
+#print Lists.Equiv.symm /-
 theorem Equiv.symm {l₁ l₂ : Lists α} (h : l₁ ~ l₂) : l₂ ~ l₁ := by
   cases' h with _ _ _ h₁ h₂ <;> [rfl, exact equiv.antisymm h₂ h₁]
 #align lists.equiv.symm Lists.Equiv.symm
+-/
 
+#print Lists.Equiv.trans /-
 theorem Equiv.trans : ∀ {l₁ l₂ l₃ : Lists α}, l₁ ~ l₂ → l₂ ~ l₃ → l₁ ~ l₃ :=
   by
   let trans := fun l₁ : Lists α => ∀ ⦃l₂ l₃⦄, l₁ ~ l₂ → l₂ ~ l₃ → l₁ ~ l₃
@@ -338,12 +421,14 @@ theorem Equiv.trans : ∀ {l₁ l₂ l₃ : Lists α}, l₁ ~ l₂ → l₂ ~ l�
   · intro a l IH₁ IH₂
     simpa [IH₁] using IH₂
 #align lists.equiv.trans Lists.Equiv.trans
+-/
 
 instance : Setoid (Lists α) :=
   ⟨(· ~ ·), Equiv.refl, @Equiv.symm _, @Equiv.trans _⟩
 
 section Decidable
 
+#print Lists.Equiv.decidableMeas /-
 @[simp]
 def Equiv.decidableMeas :
     (PSum (Σ'l₁ : Lists α, Lists α) <|
@@ -353,28 +438,48 @@ def Equiv.decidableMeas :
   | PSum.inr <| PSum.inl ⟨l₁, l₂⟩ => SizeOf.sizeOf l₁ + SizeOf.sizeOf l₂
   | PSum.inr <| PSum.inr ⟨l₁, l₂⟩ => SizeOf.sizeOf l₁ + SizeOf.sizeOf l₂
 #align lists.equiv.decidable_meas Lists.Equiv.decidableMeas
+-/
 
 open WellFoundedTactics
 
-theorem sizeOf_pos {b} (l : Lists' α b) : 0 < SizeOf.sizeOf l := by
+/- warning: lists.sizeof_pos -> Lists.sizeof_pos is a dubious translation:
+lean 3 declaration is
+  forall {α : Type.{u1}} {b : Bool} (l : Lists'.{u1} α b), LT.lt.{0} Nat Nat.hasLt (OfNat.ofNat.{0} Nat 0 (OfNat.mk.{0} Nat 0 (Zero.zero.{0} Nat Nat.hasZero))) (SizeOf.sizeOf.{succ u1} (Lists'.{u1} α b) (Lists'.hasSizeofInst.{u1} α (defaultHasSizeof.{succ u1} α) b) l)
+but is expected to have type
+  forall {α : Type.{u1}} {b : Bool} (l : Lists'.{u1} α b), LT.lt.{0} Nat instLTNat (OfNat.ofNat.{0} Nat 0 (instOfNatNat 0)) (SizeOf.sizeOf.{succ u1} (Lists'.{u1} α b) (Lists'._sizeOf_inst.{u1} α b (instSizeOf.{succ u1} α)) l)
+Case conversion may be inaccurate. Consider using '#align lists.sizeof_pos Lists.sizeof_posₓ'. -/
+theorem sizeof_pos {b} (l : Lists' α b) : 0 < SizeOf.sizeOf l := by
   cases l <;>
     run_tac
       andthen unfold_sizeof trivial_nat_lt
-#align lists.sizeof_pos Lists.sizeOf_pos
+#align lists.sizeof_pos Lists.sizeof_pos
 
+/- warning: lists.lt_sizeof_cons' -> Lists.lt_sizeof_cons' is a dubious translation:
+lean 3 declaration is
+  forall {α : Type.{u1}} {b : Bool} (a : Lists'.{u1} α b) (l : Lists'.{u1} α Bool.true), LT.lt.{0} Nat Nat.hasLt (SizeOf.sizeOf.{succ u1} (Sigma.{0, u1} Bool (fun (b : Bool) => Lists'.{u1} α b)) (Sigma.hasSizeof.{0, u1} Bool (fun (b : Bool) => Lists'.{u1} α b) Bool.hasSizeof (fun (a : Bool) => Lists'.hasSizeofInst.{u1} α (defaultHasSizeof.{succ u1} α) a)) (Sigma.mk.{0, u1} Bool (fun (b : Bool) => Lists'.{u1} α b) b a)) (SizeOf.sizeOf.{succ u1} (Lists'.{u1} α Bool.true) (Lists'.hasSizeofInst.{u1} α (defaultHasSizeof.{succ u1} α) Bool.true) (Lists'.cons'.{u1} α b a l))
+but is expected to have type
+  forall {α : Type.{u1}} {b : Bool} (a : Lists'.{u1} α b) (l : Lists'.{u1} α Bool.true), LT.lt.{0} Nat instLTNat (SizeOf.sizeOf.{succ u1} (Sigma.{0, u1} Bool (fun (b : Bool) => Lists'.{u1} α b)) (Sigma._sizeOf_inst.{0, u1} Bool (fun (b : Bool) => Lists'.{u1} α b) Bool._sizeOf_inst (fun (a : Bool) => Lists'._sizeOf_inst.{u1} α a (instSizeOf.{succ u1} α))) (Sigma.mk.{0, u1} Bool (fun (b : Bool) => Lists'.{u1} α b) b a)) (SizeOf.sizeOf.{succ u1} (Lists'.{u1} α Bool.true) (Lists'._sizeOf_inst.{u1} α Bool.true (instSizeOf.{succ u1} α)) (Lists'.cons'.{u1} α b a l))
+Case conversion may be inaccurate. Consider using '#align lists.lt_sizeof_cons' Lists.lt_sizeof_cons'ₓ'. -/
 /- ./././Mathport/Syntax/Translate/Tactic/Builtin.lean:72:18: unsupported non-interactive tactic well_founded_tactics.unfold_sizeof -/
-theorem lt_sizeOf_cons' {b} (a : Lists' α b) (l) :
+theorem lt_sizeof_cons' {b} (a : Lists' α b) (l) :
     SizeOf.sizeOf (⟨b, a⟩ : Lists α) < SizeOf.sizeOf (Lists'.cons' a l) :=
   by
   run_tac
     unfold_sizeof
   apply sizeof_pos
-#align lists.lt_sizeof_cons' Lists.lt_sizeOf_cons'
+#align lists.lt_sizeof_cons' Lists.lt_sizeof_cons'
 
 /- ./././Mathport/Syntax/Translate/Tactic/Builtin.lean:72:18: unsupported non-interactive tactic well_founded_tactics.default_dec_tac -/
 /- ./././Mathport/Syntax/Translate/Tactic/Builtin.lean:72:18: unsupported non-interactive tactic well_founded_tactics.default_dec_tac -/
 /- ./././Mathport/Syntax/Translate/Tactic/Builtin.lean:72:18: unsupported non-interactive tactic well_founded_tactics.default_dec_tac -/
+/- warning: lists.mem.decidable -> Lists.mem.decidable is a dubious translation:
+lean 3 declaration is
+  forall {α : Type.{u1}} [_inst_1 : DecidableEq.{succ u1} α] (a : Lists.{u1} α) (l : Lists'.{u1} α Bool.true), Decidable (Membership.Mem.{u1, u1} (Lists.{u1} α) (Lists'.{u1} α Bool.true) (Lists'.hasMem.{u1} α Bool.true) a l)
+but is expected to have type
+  forall {α : Type.{u1}} [_inst_1 : DecidableEq.{succ u1} α] (a : Lists.{u1} α) (l : Lists'.{u1} α Bool.true), Decidable (Membership.mem.{u1, u1} (Lists.{u1} α) (Lists'.{u1} α Bool.true) (Lists'.instMembershipListsLists'.{u1} α Bool.true) a l)
+Case conversion may be inaccurate. Consider using '#align lists.mem.decidable Lists.mem.decidableₓ'. -/
 /- ./././Mathport/Syntax/Translate/Tactic/Builtin.lean:72:18: unsupported non-interactive tactic well_founded_tactics.default_dec_tac -/
+#print Lists.Equiv.decidable /-
 mutual
   @[instance]
   def Equiv.decidable [DecidableEq α] : ∀ l₁ l₂ : Lists α, Decidable (l₁ ~ l₂)
@@ -422,7 +527,7 @@ mutual
         subset.decidable l₁ l₂
       exact decidable_of_iff' _ (@Lists'.cons_subset _ ⟨_, _⟩ _ _)
   @[instance]
-  def Mem.decidable [DecidableEq α] : ∀ (a : Lists α) (l : Lists' α true), Decidable (a ∈ l)
+  def mem.decidable [DecidableEq α] : ∀ (a : Lists α) (l : Lists' α true), Decidable (a ∈ l)
     | a, Lists'.nil => isFalse <| by rintro ⟨_, ⟨⟩, _⟩
     | a, Lists'.cons' b l₂ =>
       by
@@ -445,7 +550,8 @@ mutual
 end termination_by' ⟨_, measure_wf equiv.decidable_meas⟩
 #align lists.equiv.decidable Lists.Equiv.decidable
 #align lists.subset.decidable Lists.Subset.decidable
-#align lists.mem.decidable Lists.Mem.decidable
+#align lists.mem.decidable Lists.mem.decidable
+-/
 
 end Decidable
 
@@ -453,24 +559,40 @@ end Lists
 
 namespace Lists'
 
+/- warning: lists'.mem_equiv_left -> Lists'.mem_equiv_left is a dubious translation:
+lean 3 declaration is
+  forall {α : Type.{u1}} {l : Lists'.{u1} α Bool.true} {a : Lists.{u1} α} {a' : Lists.{u1} α}, (Lists.Equiv.{u1} α a a') -> (Iff (Membership.Mem.{u1, u1} (Lists.{u1} α) (Lists'.{u1} α Bool.true) (Lists'.hasMem.{u1} α Bool.true) a l) (Membership.Mem.{u1, u1} (Lists.{u1} α) (Lists'.{u1} α Bool.true) (Lists'.hasMem.{u1} α Bool.true) a' l))
+but is expected to have type
+  forall {α : Type.{u1}} {l : Lists'.{u1} α Bool.true} {a : Lists.{u1} α} {a' : Lists.{u1} α}, (Lists.Equiv.{u1} α a a') -> (Iff (Membership.mem.{u1, u1} (Lists.{u1} α) (Lists'.{u1} α Bool.true) (Lists'.instMembershipListsLists'.{u1} α Bool.true) a l) (Membership.mem.{u1, u1} (Lists.{u1} α) (Lists'.{u1} α Bool.true) (Lists'.instMembershipListsLists'.{u1} α Bool.true) a' l))
+Case conversion may be inaccurate. Consider using '#align lists'.mem_equiv_left Lists'.mem_equiv_leftₓ'. -/
 theorem mem_equiv_left {l : Lists' α true} : ∀ {a a'}, a ~ a' → (a ∈ l ↔ a' ∈ l) :=
   suffices ∀ {a a'}, a ~ a' → a ∈ l → a' ∈ l from fun a a' e => ⟨this e, this e.symm⟩
   fun a₁ a₂ e₁ ⟨a₃, m₃, e₂⟩ => ⟨_, m₃, e₁.symm.trans e₂⟩
 #align lists'.mem_equiv_left Lists'.mem_equiv_left
 
+/- warning: lists'.mem_of_subset -> Lists'.mem_of_subset is a dubious translation:
+lean 3 declaration is
+  forall {α : Type.{u1}} {a : Lists.{u1} α} {l₁ : Lists'.{u1} α Bool.true} {l₂ : Lists'.{u1} α Bool.true}, (HasSubset.Subset.{u1} (Lists'.{u1} α Bool.true) (Lists'.hasSubset.{u1} α) l₁ l₂) -> (Membership.Mem.{u1, u1} (Lists.{u1} α) (Lists'.{u1} α Bool.true) (Lists'.hasMem.{u1} α Bool.true) a l₁) -> (Membership.Mem.{u1, u1} (Lists.{u1} α) (Lists'.{u1} α Bool.true) (Lists'.hasMem.{u1} α Bool.true) a l₂)
+but is expected to have type
+  forall {α : Type.{u1}} {a : Lists.{u1} α} {l₁ : Lists'.{u1} α Bool.true} {l₂ : Lists'.{u1} α Bool.true}, (HasSubset.Subset.{u1} (Lists'.{u1} α Bool.true) (Lists'.instHasSubsetLists'True.{u1} α) l₁ l₂) -> (Membership.mem.{u1, u1} (Lists.{u1} α) (Lists'.{u1} α Bool.true) (Lists'.instMembershipListsLists'.{u1} α Bool.true) a l₁) -> (Membership.mem.{u1, u1} (Lists.{u1} α) (Lists'.{u1} α Bool.true) (Lists'.instMembershipListsLists'.{u1} α Bool.true) a l₂)
+Case conversion may be inaccurate. Consider using '#align lists'.mem_of_subset Lists'.mem_of_subsetₓ'. -/
 theorem mem_of_subset {a} {l₁ l₂ : Lists' α true} (s : l₁ ⊆ l₂) : a ∈ l₁ → a ∈ l₂
   | ⟨a', m, e⟩ => (mem_equiv_left e).2 (mem_of_subset' s m)
 #align lists'.mem_of_subset Lists'.mem_of_subset
 
+#print Lists'.Subset.trans /-
 theorem Subset.trans {l₁ l₂ l₃ : Lists' α true} (h₁ : l₁ ⊆ l₂) (h₂ : l₂ ⊆ l₃) : l₁ ⊆ l₃ :=
   subset_def.2 fun a₁ m₁ => mem_of_subset h₂ <| mem_of_subset' h₁ m₁
 #align lists'.subset.trans Lists'.Subset.trans
+-/
 
 end Lists'
 
+#print Finsets /-
 def Finsets (α : Type _) :=
   Quotient (@Lists.setoid α)
 #align finsets Finsets
+-/
 
 namespace Finsets
 
