Mathbin/Tactic/RewriteSearch/Discovery.lean
@@ -99,7 +99,7 @@ private unsafe def rewrites_for_rule (exp : expr) (cfg : config) (numbered_rule 
 unsafe def get_rewrites (rules : List (expr × Bool)) (exp : expr) (cfg : config) :
     tactic (Buffer rewrite) := do
   let lists ← List.mapM (rewrites_for_rule exp cfg) rules.enum
-  return (List.foldl Buffer.appendList Buffer.nil lists)
+  return (List.foldl Buffer.appendList Buffer.nil Lists)
 #align tactic.rewrite_search.get_rewrites tactic.rewrite_search.get_rewrites
 
 end Tactic.RewriteSearch
